---
Last time checked: 2024-01-26
Complete: true
aliases:
---
# First isomorphism theorem
***
###### tags: #Algebra 
***
#### For rings
>[!dsn]+ Theorem
>Let $f:R\to S$ be a surjective ring homomorphism. Then $S\cong R/\ker{f}$.^[[Lectures at KAU - Yevgen Polulyakh 7](https://drive.google.com/drive/folders/1OBF4iFXhiyJQ2lVaDTRnDEnyDf6hImIg)]

>If fact $f$ induces isomorphism $\tilde{f}:R/\ker{f}\;\tilde\to\; S$ defined by $\tilde{f}(a+\ker{f})=f(a)$.

>[!proof]+
>By the [[canonical map decomposition]] for rings, $R/\ker{f}\cong f(R)$, and the isomorphism $\tilde{f}$ is defined by $a+\ker{f}\mapsto f(a)$. Since $f$ is surjective, $f(R)=S$. The statement follows immediately.

>[!example]+ 
>Let $R$ be a commutative ring, $r\in R$. Consider the evaluation map $e_{r}:R[x]\to R$, $\forall f\in R[x]$, $e_{r}:f\mapsto\hat{f}(r)$.
>
>$e_{r}$ is surjective, as $e_{r}(s+0\cdot x+\dots)=s$, $\forall s\in R$.
>Denote $\forall s\in R$, $f(s)=\hat{f}(s)+0x+0x^{2}+\dots$. Then
>$$\ker{e_{r}}=\left\{f\in R[x]:\hat{f}(R)=0 \right\}=\{f\in R[x]:f(r)=0 \}$$
>Let $f\in R[x]$, $r\in R$. Then $\exists q\in R[x]$, such that $f(x)=(x-r)q(x)+f(r)$
>>[!proof]+
>>Let $f=a_{0}+a_{1}x+\dots+a_{n}x^{n}$. Then polynomial $f-f(0)$ is divisible by $x$, that is $f-f(0)\in\langle x \rangle$ (principal ideal generated by $x$). 
>>Make a *change of variable* $x=t+r$. Consider a polynomial $g(t)$ with respect to $t$.
>>$$g(t)=f(t+r)=a_{0}+a_{1}(t+r)+\dots+a_{n}(t+r)^{n}$$
>>Then $g-g(0)$ is divisible by $t$. But $g(0)=f(r)$, so $g-f(r)$ is divisible by $t=x-r$.
>>Next $\hat{f}(r)=0\Leftrightarrow(x-r)q(x)$ for some $q(x)\in R[x]$. Thus $\ker{e_{r}}=\langle x-r\rangle$. By [[First isomorphism theorem]] we have that
>>$$R[x]/\langle x-r \rangle\cong R$$

***
#### Keywords
- [[Ring]],
- [[Homomorphism]],
- [[Isomorphism]],
- [[Quotient set]],
- [[Kernel and image of a mapping]],
- [[Commutative property]],
- [[Evaluation map]],
- [[Polynomial]],
- [[Principal ideal]],
- [[Divisibility]]
#### Possibly related
- 
***
#### Sources: